MatrixMortality/PrefixContextsNonsingular.lean
@@ -1,4 +1,4 @@
-import MatrixMortality.PrefixAlgebraContexts
+import MatrixMortality.PrefixContextsClosed
 
 /-!
 # Nonsingularity of the ten-state prefix contexts
@@ -12,7 +12,7 @@ block and ends with one pivot.
 namespace MatrixMortality
 
 open scoped Matrix
-open PrefixAlgebra.Certificate
+open PrefixContexts.Certificate
 
 attribute [local simp]
   vecCons_val_three vecCons_val_four vecCons_val_five vecCons_val_six
